lib/Lib.ByteSequence.fst
@@ -116,43 +116,48 @@ let nat_from_bytes_le = nat_from_intseq_le #U8
 
 #set-options "--max_fuel 1"
 
-val nat_to_bytes_be_:
-    #l:secrecy_level
+val nat_to_intseq_be_:
+    #t:inttype -> #l:secrecy_level
   -> len:nat
-  -> n:nat{ n < pow2 (8 * len)}
-  -> Tot (b:bytes_l l {length b == len /\ n == nat_from_intseq_be #U8 b}) (decreases len)
-let rec nat_to_bytes_be_ #l len n =
-  if len = 0 then create len (uint #U8 #l 0)
+  -> n:nat{n < pow2 (bits t * len)}
+  -> Tot (b:seq (uint_t t l){length b == len /\ n == nat_from_intseq_be b}) (decreases len)
+let rec nat_to_intseq_be_ #t #l len n =
+  if len = 0 then create len (uint #t #l 0)
   else
     let len' = len - 1 in
-    let byte = uint #U8 #l (n % 256) in
-    let n' = n / 256 in
-    Math.Lemmas.pow2_plus 8 (8 * len');
-    let b' = nat_to_bytes_be_ len' n' in
-    let b  = Seq.append b' (create 1 byte) in
-    Seq.append_slices b' (create 1 byte);
+    let tt = uint #t #l (n % modulus t) in
+    let n' = n / modulus t in
+    assert (modulus t = pow2 (bits t));
+    FStar.Math.Lemmas.lemma_div_lt_nat n (bits t * len) (bits t);
+    let b' = nat_to_intseq_be_ len' n' in
+    let b  = Seq.append b' (create 1 tt) in
+    Seq.append_slices b' (create 1 tt);
     b
 
-let nat_to_bytes_be = nat_to_bytes_be_
+let nat_to_intseq_be = nat_to_intseq_be_
 
-val nat_to_bytes_le_:
-    #l:secrecy_level
+val nat_to_intseq_le_:
+    #t:inttype -> #l:secrecy_level
   -> len:nat
-  -> n:nat{n < pow2 (8 * len)}
-  -> Tot (b:bytes_l l {length b == len /\ n == nat_from_intseq_le b}) (decreases len)
-let rec nat_to_bytes_le_ #l len n =
-  if len = 0 then create len (uint #U8 #l 0)
+  -> n:nat{n < pow2 (bits t * len)}
+  -> Tot (b:seq (uint_t t l){length b == len /\ n == nat_from_intseq_le b}) (decreases len)
+let rec nat_to_intseq_le_ #t #l len n =
+  if len = 0 then create len (uint #t #l 0)
   else
     let len' = len - 1 in
-    let byte = uint #U8 #l (n % 256) in
-    let n' = n / 256 in
-    Math.Lemmas.pow2_plus 8 (8 * len');
-    let b' = nat_to_bytes_le_ #l len' n' in
-    let b = Seq.append (create 1 byte) b' in
-    Seq.append_slices (create 1 byte) b';
+    let tt = uint #t #l (n % modulus t) in
+    let n' = n / modulus t in
+    assert (modulus t = pow2 (bits t));
+    FStar.Math.Lemmas.lemma_div_lt_nat n (bits t * len) (bits t);
+    let b' = nat_to_intseq_le_ len' n' in
+    let b = Seq.append (create 1 tt) b' in
+    Seq.append_slices (create 1 tt) b';
     b
 
-let nat_to_bytes_le = nat_to_bytes_le_
+let nat_to_intseq_le = nat_to_intseq_le_
+
+let nat_to_bytes_be = nat_to_intseq_be_ #U8
+let nat_to_bytes_le = nat_to_intseq_le_ #U8
 
 val index_nat_to_bytes_le:
     #l:secrecy_level
@@ -225,3 +230,125 @@ let uints_from_bytes_le #t #l #len b =
 let uints_from_bytes_be #t #l #len b =
   Lib.Sequence.createi #(uint_t t l) len
     (fun i -> uint_from_bytes_be (sub b (i * numbytes t) (numbytes t)))
+
+val nat_from_intseq_le_slice_lemma0:
+  #t:inttype -> #l:secrecy_level -> #len:size_nat{len > 0} -> b:lseq (uint_t t l) len -> i:size_nat{0 < i /\ i <= len} ->
+  Lemma
+    (pow2 ((i - 1) * bits t) * nat_from_intseq_le_ (Seq.slice b (i - 1) len) ==
+     pow2 ((i - 1) * bits t) * v b.[i - 1] + pow2 (i * bits t) * nat_from_intseq_le_ (Seq.slice b i len))
+let nat_from_intseq_le_slice_lemma0 #t #l #len b i =
+  FStar.Math.Lemmas.distributivity_add_right (pow2 ((i - 1) * bits t)) (v b.[i - 1]) (pow2 (bits t) * nat_from_intseq_le_ (Seq.slice b i len));
+  FStar.Math.Lemmas.paren_mul_right (pow2 ((i - 1) * bits t)) (pow2 (bits t)) (nat_from_intseq_le_ (Seq.slice b i len));
+  FStar.Math.Lemmas.pow2_plus ((i - 1) * bits t) (bits t)
+
+val nat_from_intseq_le_slice_lemma1:
+  #t:inttype -> #l:secrecy_level -> #len:size_nat -> b:lseq (uint_t t l) len -> i:size_nat{0 < i /\ i <= len} ->
+  Lemma
+    (requires (let b1 = Seq.slice b 0 i in
+      nat_from_intseq_le_ b1 == nat_from_intseq_le_ (Seq.slice b1 0 (i - 1)) + pow2 ((i - 1) * bits t) * nat_from_intseq_le_ (Seq.slice b1 (i - 1) i)))
+    (ensures
+      nat_from_intseq_le_ (Seq.slice b 0 i) == nat_from_intseq_le_ (Seq.slice b 0 (i - 1)) + pow2 ((i - 1) * bits t) * v b.[i - 1])
+let nat_from_intseq_le_slice_lemma1 #t #l #len b i = ()
+
+val nat_from_intseq_le_slice_lemma_:
+  #t:inttype -> #l:secrecy_level -> #len:size_nat -> b:lseq (uint_t t l) len -> i:nat{i <= len} ->
+  Lemma
+    (nat_from_intseq_le_ b == nat_from_intseq_le_ (Seq.slice b 0 i) + pow2 (i * bits t) * nat_from_intseq_le_ (Seq.slice b i len))
+let rec nat_from_intseq_le_slice_lemma_ #t #l #len b i =
+  if len = 0 then ()
+  else begin
+    if i = 0 then ()
+    else begin
+      nat_from_intseq_le_slice_lemma_ b (i - 1);
+      nat_from_intseq_le_slice_lemma0 b i;
+      nat_from_intseq_le_slice_lemma_ #t #l #i (Seq.slice b 0 i) (i - 1);
+      nat_from_intseq_le_slice_lemma1 b i
+    end
+  end
+
+let nat_from_intseq_le_slice_lemma #t #l #len b i = nat_from_intseq_le_slice_lemma_ b i
+let nat_from_bytes_le_slice_lemma #l #len b i = nat_from_intseq_le_slice_lemma_ b i
+
+
+val uints_from_bytes_le_lemma0:
+    #t:inttype{~(t == U1)}
+  -> #l:secrecy_level
+  -> #len:size_nat{len * numbytes t < pow2 32}
+  -> b:lbytes_l l (len * numbytes t) ->
+  Lemma (forall (i:nat). i < len - 1 ==>
+    (uints_from_bytes_le #t #l #len b).[i + 1] == uint_from_bytes_le (sub b ((i + 1) * numbytes t) (numbytes t)))
+let uints_from_bytes_le_lemma0 #t #l #len b = ()
+
+val uints_from_bytes_le_lemma1:
+    #t:inttype{~(t == U1)}
+  -> #l:secrecy_level
+  -> #len:size_nat{0 < len /\ len * numbytes t < pow2 32}
+  -> b:lbytes_l l (len * numbytes t) ->
+  Lemma (forall (i:nat). i < len - 1 ==>
+    Seq.index (Seq.slice (uints_from_bytes_le #t #l #len b) 1 len) i ==
+    uint_from_bytes_le (sub b ((i + 1) * numbytes t) (numbytes t)))
+let uints_from_bytes_le_lemma1 #t #l #len b =
+  uints_from_bytes_le_lemma0 b
+
+#set-options "--z3rlimit 300"
+
+val uints_from_bytes_le_slice_lemma:
+    #t:inttype{~(t == U1)}
+  -> #l:secrecy_level
+  -> #len:size_nat{0 < len /\ len * numbytes t < pow2 32}
+  -> b:lbytes_l l (len * numbytes t) ->
+  Lemma (
+    Seq.slice (uints_from_bytes_le #t #_ #len b) 1 len ==
+    uints_from_bytes_le #t #_ #(len-1) (Seq.slice b (numbytes t) (len * numbytes t)))
+let uints_from_bytes_le_slice_lemma #t #l #len b =
+  let r = uints_from_bytes_le #t #_ #len b in
+  let r1 = uints_from_bytes_le #t #_ #(len-1) (Seq.slice b (numbytes t) (len * numbytes t)) in
+  assert (forall (i:nat). i < len - 1 ==> r1.[i] == uint_from_bytes_le (sub b ((i + 1) * numbytes t) (numbytes t)));
+  uints_from_bytes_le_lemma1 b;
+  eq_intro (Seq.slice r 1 len) r1
+
+val uints_from_bytes_le_nat_lemma0:
+    #t:inttype{~(t == U1)}
+  -> #l:secrecy_level
+  -> #len:size_nat{0 < len /\ len * numbytes t < pow2 32}
+  -> b:lbytes_l l (len * numbytes t) ->
+  Lemma (
+    nat_from_intseq_le_ (uints_from_bytes_le #t #_ #len b) ==
+    nat_from_intseq_le_ (Seq.slice b 0 (numbytes t)) +
+    pow2 (bits t) * nat_from_intseq_le_ (uints_from_bytes_le #t #_ #(len-1) (Seq.slice b (numbytes t) (numbytes t * len))))
+let uints_from_bytes_le_nat_lemma0 #t #l #len b =
+  let r = uints_from_bytes_le #t #_ #len b in
+  let r2 = Seq.slice r 1 len in
+  let b1 = Seq.slice b (numbytes t) (numbytes t * len) in
+  let r1 = uints_from_bytes_le #t #_ #(len-1) b1 in
+  uints_from_bytes_le_slice_lemma b;
+  assert (nat_from_intseq_le_ r == v r.[0] + pow2 (bits t) * nat_from_intseq_le_ r2);
+  assert (nat_from_intseq_le_ (Seq.slice b 0 (numbytes t)) == v r.[0])
+
+val uints_from_bytes_le_nat_lemma_:
+    #t:inttype{~(t == U1)}
+  -> #l:secrecy_level
+  -> #len:size_nat{len * numbytes t < pow2 32}
+  -> b:lbytes_l l (len * numbytes t) ->
+  Lemma (nat_from_intseq_le_ (uints_from_bytes_le #t #l #len b) == nat_from_intseq_le_ b)
+let rec uints_from_bytes_le_nat_lemma_ #t #l #len b =
+  if len = 0 then ()
+  else begin
+    let b1 = Seq.slice b (numbytes t) (len * numbytes t) in
+    uints_from_bytes_le_nat_lemma_ #t #l #(len - 1) b1;
+    nat_from_bytes_le_slice_lemma #l #(len * numbytes t) b (numbytes t);
+    uints_from_bytes_le_nat_lemma0 b
+  end
+
+let uints_from_bytes_le_nat_lemma #t #l #len b = uints_from_bytes_le_nat_lemma_ #t #l #len b
+
+let uints_to_bytes_le_nat_lemma #t #l len n = admit()
+
+let rec nat_from_intseq_le_inj #t #l b1 b2 =
+  if length b1 = 0 then ()
+  else begin
+    nat_from_intseq_le_inj (Seq.slice b1 1 (length b1)) (Seq.slice b2 1 (length b2));
+    Seq.lemma_split b1 1;
+    Seq.lemma_split b2 1;
+    uintv_extensionality (Seq.index b1 0) (Seq.index b2 0)
+  end
